Simple first start by showing the properties of Fifo1.

Fifo/Proofs.v
@@ -7,6 +7,364 @@ Require Import Kami.GallinaModules.Relations.
 Require Import Kami.GallinaModules.AuxLemmas.
 Require Import Kami.GallinaModules.AuxTactics.
 
+Local Definition isEmpty_impl1 (varName : string) :=
+  (Read val : Bool <- varName; Ret (! Var type (SyntaxKind Bool) val))%kami_action.
+
+Local Definition isFull_impl1 (varName : string) :=
+  (Read val : Bool <- varName; Ret Var type (SyntaxKind Bool) val)%kami_action.
+
+Local Definition numFree_impl1 (varName : string) (size' : nat) :=
+  (Read val : Bool <- varName;
+   Ret (IF Var type (SyntaxKind Bool) val
+        then Const type (natToWord size' 0)
+        else Const type $ (1)%word))%kami_action.
+
+Local Definition first_impl1 (k : Kind) (bvarName dvarName : string)  :=
+(Read val : Bool <- bvarName;
+ Read dat : k <- dvarName;
+ Ret (STRUCT {"valid" ::= Var type (SyntaxKind Bool) val;
+              "data" ::= Var type (SyntaxKind k) dat}:
+      Expr type (SyntaxKind (Maybe k))))%kami_action.  
+
+Local Definition deq_impl1 (k : Kind) (bvarName dvarName : string) :=
+(Read val : Bool <- bvarName;
+ Read dat : k <- dvarName;
+ Write bvarName : Bool <- Const type false;
+ Ret (STRUCT {"valid" ::= Var type (SyntaxKind Bool) val;
+              "data" ::= Var _ (SyntaxKind k) dat}:
+        Expr _ (SyntaxKind (Maybe k))))%kami_action.
+
+Local Definition enq_impl1 (k : Kind) (bvarName dvarName : string) (new : type k) :=
+  (Read val : Bool <- bvarName;
+   Read dat : k <- dvarName;
+   Write bvarName : Bool <- Const type true;
+   Write dvarName : k <-
+                    IF ! Var type (SyntaxKind Bool) val
+                    then Var _ (SyntaxKind k) new
+                    else Var _ _ dat;
+   Ret (! Var _ (SyntaxKind Bool) val))%kami_action.
+
+Local Definition flush_impl1 (varName : string) :=
+(Write varName : Bool <- Const type false; Retv)%kami_action.
+
+Local Lemma isEmpty1_Effectless varName val :
+  forall o reads upds calls retV,
+    NoDup (map fst o) ->
+    In (varName, existT _ (SyntaxKind Bool) val) o ->
+    SemAction o (isEmpty_impl1 varName) reads upds calls retV ->
+    upds = nil /\
+    calls = nil /\
+    retV = negb val.
+Proof.
+  unfold isEmpty_impl1; intros.
+  apply inversionSemAction in H1; dest; subst.
+  apply inversionSemAction in H2; dest; subst.
+  repeat split; auto.
+  enough ( x = val).
+  { subst; auto. }
+  specialize (NoDup_map_fst H H0 H1) as P; EqDep_subst; reflexivity.
+Qed.
+
+Local Lemma isEmpty1_Wb varName :
+  ActionWb [(varName, SyntaxKind Bool)] (isEmpty_impl1 varName).
+Proof.
+  unfold isEmpty_impl1.
+  repeat intro.
+  rewrite SubList_map_iff in H0; dest.
+  apply inversionSemAction in H1; dest; subst.
+  apply inversionSemAction in H3; dest; subst.
+  assert (SubList [(varName, existT (fullType type) (SyntaxKind Bool) x0)] o).
+  { repeat intro.
+    inv H3; [|inv H4]; assumption. }
+  specialize (SubList_chain H H0 H3) as P.
+  rewrite <- fst_getKindAttr in P.
+  setoid_rewrite H2 in P.
+  rewrite (P (eq_refl _)) in *.
+  split.
+  - exists [(varName, existT _ (SyntaxKind Bool) x0)]; repeat split; auto.
+    + apply SubList_refl.
+    + repeat econstructor.
+  - apply SubList_nil_l.
+Qed.
+
+Local Lemma isFull1_Effectless varName val :
+  forall o reads upds calls retV,
+    NoDup (map fst o) ->
+    In (varName, existT _ (SyntaxKind Bool) val) o ->
+    SemAction o (isFull_impl1 varName) reads upds calls retV ->
+    upds = nil /\
+    calls = nil /\
+    retV = val.
+Proof.
+  unfold isFull_impl1; intros.
+  apply inversionSemAction in H1; dest; subst.
+  apply inversionSemAction in H2; dest; subst.
+  repeat split; auto.
+  enough ( x = val).
+  { subst; auto. }
+  specialize (NoDup_map_fst H H0 H1) as P; EqDep_subst; reflexivity.
+Qed.
+
+Local Lemma isFull1_Wb varName :
+  ActionWb [(varName, SyntaxKind Bool)] (isFull_impl1 varName).
+Proof.
+  unfold isFull_impl1.
+  repeat intro.
+  rewrite SubList_map_iff in H0; dest.
+  apply inversionSemAction in H1; dest; subst.
+  apply inversionSemAction in H3; dest; subst.
+  assert (SubList [(varName, existT (fullType type) (SyntaxKind Bool) x0)] o).
+  { repeat intro.
+    inv H3; [|inv H4]; assumption. }
+  specialize (SubList_chain H H0 H3) as P.
+  rewrite <- fst_getKindAttr in P.
+  setoid_rewrite H2 in P.
+  rewrite (P (eq_refl _)) in *.
+  split.
+  - exists [(varName, existT _ (SyntaxKind Bool) x0)]; repeat split; auto.
+    + apply SubList_refl.
+    + repeat econstructor.
+  - apply SubList_nil_l.
+Qed.
+
+Local Lemma numFree1_Effectless varName size' val :
+  forall o reads upds calls retV,
+    NoDup (map fst o) ->
+    In (varName, existT _ (SyntaxKind Bool) val) o ->
+    SemAction o (numFree_impl1 varName size') reads upds calls retV ->
+    upds = nil /\
+    calls = nil /\
+    retV = (if val then (natToWord size' 0) else (natToWord size' 1)).
+Proof.
+  unfold numFree_impl1; intros.
+  apply inversionSemAction in H1; dest; subst.
+  apply inversionSemAction in H2; dest; subst.
+  repeat split; auto.
+  enough ( x = val).
+  { subst; auto. }
+  specialize (NoDup_map_fst H H0 H1) as P; EqDep_subst; reflexivity.
+Qed.
+
+Local Lemma numFree1_Wb varName size' :
+  ActionWb [(varName, SyntaxKind Bool)] (numFree_impl1 varName size').
+Proof.
+  unfold numFree_impl1.
+  repeat intro.
+  rewrite SubList_map_iff in H0; dest.
+  apply inversionSemAction in H1; dest; subst.
+  apply inversionSemAction in H3; dest; subst.
+  assert (SubList [(varName, existT (fullType type) (SyntaxKind Bool) x0)] o).
+  { repeat intro.
+    inv H3; [|inv H4]; assumption. }
+  specialize (SubList_chain H H0 H3) as P.
+  rewrite <- fst_getKindAttr in P.
+  setoid_rewrite H2 in P.
+  rewrite (P (eq_refl _)) in *.
+  split.
+  - exists [(varName, existT _ (SyntaxKind Bool) x0)]; repeat split; auto.
+    + apply SubList_refl.
+    + repeat econstructor.
+  - apply SubList_nil_l.
+Qed.
+
+Local Lemma first1_Effectless k bvarName dvarName bval dval:
+  forall o reads upds calls retV,
+    NoDup (map fst o) ->
+    In (bvarName, existT _ (SyntaxKind Bool) bval) o ->
+    In (dvarName, existT _ (SyntaxKind k) dval) o ->
+    SemAction o (first_impl1 k bvarName dvarName) reads upds calls retV ->
+    upds = nil /\
+    calls = nil /\
+    (retV F1 = bval) /\
+    (retV (FS F1) = dval).
+Proof.
+  unfold first_impl1; intros.
+  apply inversionSemAction in H2; dest; subst.
+  apply inversionSemAction in H3; dest; subst.
+  apply inversionSemAction in H4; dest; subst.
+  repeat split; auto.
+  - specialize (NoDup_map_fst H H0 H2) as P; EqDep_subst; reflexivity.
+  - specialize (NoDup_map_fst H H1 H3) as P; EqDep_subst; reflexivity.
+Qed.
+
+Local Lemma first1_Wb k bvarName dvarName :
+  ActionWb [(bvarName, SyntaxKind Bool); (dvarName, SyntaxKind k)]
+           (first_impl1 k bvarName dvarName).
+Proof.
+  unfold first_impl1.
+  repeat intro.
+  rewrite SubList_map_iff in H0; dest.
+  apply inversionSemAction in H1; dest; subst.
+  apply inversionSemAction in H3; dest; subst.
+  apply inversionSemAction in H4; dest; subst.
+  split; [|apply SubList_nil_l].
+  exists x.
+  assert (SubList [(bvarName, existT _ (SyntaxKind Bool) x0);
+                   (dvarName, existT _ (SyntaxKind k) x2)] o).
+  { repeat intro.
+    inv H4; [|inv H5; [|inv H4]]; assumption. }
+  specialize (SubList_chain H H0 H4) as P.
+  rewrite <- fst_getKindAttr in P.
+  setoid_rewrite H2 in P.
+  rewrite (P (eq_refl _)) in *.
+  repeat split; auto.
+  - apply SubList_refl.
+  - econstructor; eauto.
+    + left; reflexivity.
+    + econstructor; eauto.
+      * right; left; reflexivity.
+      * econstructor; eauto.
+Qed.
+
+Local Lemma deq1_Effectful k bvarName dvarName bval dval :
+  forall o reads upds calls retV,
+    NoDup (map fst o) ->
+    In (bvarName, existT _ (SyntaxKind Bool) bval) o ->
+    In (dvarName, existT _ (SyntaxKind k) dval) o ->
+    SemAction o (deq_impl1 k bvarName dvarName) reads upds calls retV ->
+    upds = [(bvarName, existT _ (SyntaxKind Bool) false)] /\
+    calls = nil /\
+    (retV F1 = bval) /\
+    (retV (FS F1) = dval).
+Proof.
+  unfold deq_impl1; intros.
+  apply inversionSemAction in H2; dest; subst.
+  apply inversionSemAction in H3; dest; subst.
+  apply inversionSemAction in H4; dest; subst.
+  apply inversionSemAction in H6; dest; subst.
+  repeat split; auto.
+  - specialize (NoDup_map_fst H H0 H2) as P; EqDep_subst; reflexivity.
+  - specialize (NoDup_map_fst H H1 H3) as P; EqDep_subst; reflexivity.
+Qed.
+
+Local Lemma deq1_Wb k bvarName dvarName :
+  ActionWb [(bvarName, SyntaxKind Bool); (dvarName, SyntaxKind k)]
+           (deq_impl1 k bvarName dvarName).
+Proof.
+  unfold deq_impl1.
+  repeat intro.
+  rewrite SubList_map_iff in H0; dest.
+  apply inversionSemAction in H1; dest; subst.
+  apply inversionSemAction in H3; dest; subst.
+  apply inversionSemAction in H4; dest; subst.
+  apply inversionSemAction in H6; dest; subst.
+  split.
+  - exists x.
+    assert (SubList [(bvarName, existT _ (SyntaxKind Bool) x0);
+                     (dvarName, existT _ (SyntaxKind k) x2)] o).
+    { repeat intro.
+      inv H6; [|inv H7; [|inv H6]]; assumption. }
+  specialize (SubList_chain H H0 H6) as P.
+  rewrite <- fst_getKindAttr in P.
+  setoid_rewrite H2 in P.
+  rewrite (P (eq_refl _)) in *.
+  repeat split; auto.
+    + apply SubList_refl.
+    + econstructor; eauto.
+      * left; reflexivity.
+      * econstructor; eauto.
+        -- right; left; reflexivity.
+        -- econstructor; eauto.
+           ++ left; auto.
+           ++ econstructor; eauto.
+  - repeat intro; inv H6;[|inv H7].
+    left; reflexivity.
+Qed.
+
+Local Lemma eqn1_Effectful k bvarName dvarName bval dval new:
+  forall o reads upds calls retV,
+    NoDup (map fst o) ->
+    In (bvarName, existT _ (SyntaxKind Bool) bval) o ->
+    In (dvarName, existT _ (SyntaxKind k) dval) o ->
+    SemAction o (enq_impl1 k bvarName dvarName new) reads upds calls retV ->
+    upds = [(bvarName, existT _ (SyntaxKind Bool) true);
+           (dvarName, existT _ (SyntaxKind k) 
+                             (if (negb bval)
+                             then new
+                             else dval))] /\
+    calls = nil /\
+    (retV = negb bval).
+Proof.
+  unfold enq_impl1; intros.
+  apply inversionSemAction in H2; dest; subst.
+  apply inversionSemAction in H3; dest; subst.
+  apply inversionSemAction in H4; dest; subst.
+  apply inversionSemAction in H6; dest; subst.
+  apply inversionSemAction in H8; dest; subst.
+  specialize (NoDup_map_fst H H0 H2) as P; EqDep_subst;
+    specialize (NoDup_map_fst H H1 H3) as P1; EqDep_subst.
+  repeat split; auto.
+Qed.
+
+Local Lemma eqn1_Wb k bvarName dvarName new:
+  ActionWb [(bvarName, SyntaxKind Bool); (dvarName, SyntaxKind k)]
+           (enq_impl1 k bvarName dvarName new).
+Proof.
+  unfold enq_impl1.
+  repeat intro.
+  rewrite SubList_map_iff in H0; dest.
+  apply inversionSemAction in H1; dest; subst.
+  apply inversionSemAction in H3; dest; subst.
+  apply inversionSemAction in H4; dest; subst.
+  apply inversionSemAction in H6; dest; subst.
+  apply inversionSemAction in H8; dest; subst.
+  split.
+  - exists x.
+    assert (SubList [(bvarName, existT _ (SyntaxKind Bool) x0);
+                     (dvarName, existT _ (SyntaxKind k) x2)] o).
+    { repeat intro.
+      inv H8; [|inv H9; [|inv H8]]; assumption. }
+  specialize (SubList_chain H H0 H8) as P.
+  rewrite <- fst_getKindAttr in P.
+  setoid_rewrite H2 in P.
+  rewrite (P (eq_refl _)) in *.
+  repeat split; auto.
+    + apply SubList_refl.
+    + econstructor; eauto.
+      * left; reflexivity.
+      * econstructor; eauto.
+        -- right; left; reflexivity.
+        -- econstructor; eauto.
+           ++ left; auto.
+           ++ econstructor; eauto.
+              ** right; left; reflexivity.
+              ** econstructor; reflexivity.
+  - repeat intro; inv H8;[|inv H9; [|inv H8]].
+    + left; reflexivity.
+    + right; left; reflexivity.
+Qed.
+
+Local Lemma flush1_Effectful varName :
+  forall o reads upds calls retV,
+    SemAction o (flush_impl1 varName) reads upds calls retV ->
+    upds = [(varName, existT _ (SyntaxKind Bool) false)] /\
+    calls = nil /\
+    (retV = WO).
+Proof.
+  unfold flush_impl1; intros.
+  apply inversionSemAction in H; dest; subst.
+  apply inversionSemAction in H1; dest; subst.
+  repeat split; auto.
+Qed.
+
+Local Lemma flush_Wb varName:
+  ActionWb [(varName, SyntaxKind Bool)]
+           (flush_impl1 varName).
+Proof.
+  unfold flush_impl1.
+  repeat intro.
+  rewrite SubList_map_iff in H0; dest.
+  apply inversionSemAction in H1; dest; subst.
+  apply inversionSemAction in H4; dest; subst.
+  split; [|apply SubList_refl].
+  exists x.
+  repeat split; auto.
+  - apply SubList_nil_l.
+  - repeat econstructor; eauto.
+    rewrite H2.
+    left; reflexivity.
+Qed.
+
 Record FifoCorrect {FParams} (imp spec : @Fifo.Ifc.Ifc FParams) : Type :=
   {
     fifoRegs : list (Attribute FullKind);
@@ -17,13 +375,13 @@ Record FifoCorrect {FParams} (imp spec : @Fifo.Ifc.Ifc FParams) : Type :=
     isFullWb : ActionWb fifoRegs (@isFull _ imp type);
     numFreeCorrect : EffectlessRelation fifoR (@numFree _ imp type) (@numFree _ spec type);
     numFreeWb : ActionWb fifoRegs (@numFree _ imp type);
-    firstCorrect : EffectfulRelation fifoR (@first _ imp type) (@first _ spec type);
+    firstCorrect : EffectlessRelation fifoR (@first _ imp type) (@first _ spec type);
     firstWb : ActionWb fifoRegs (@first _ imp type);
     deqCorrect : EffectfulRelation fifoR (@deq _ imp type) (@deq _ spec type);
     deqWb : ActionWb fifoRegs (@deq _ imp type);
     enqCorrect : forall val, EffectfulRelation fifoR (@enq _ imp type val) (@enq _ spec type val);
     enqWb : forall val, ActionWb fifoRegs (@enq _ imp type val);
-    flushCorrect : EffectlessRelation fifoR (@flush _ imp type) (@flush _ spec type);
+    flushCorrect : EffectfulRelation fifoR (@flush _ imp type) (@flush _ spec type);
   }.
 
 Section Proofs.
